compiler/lib/ast_to_sexp.mli
@@ -56,8 +56,8 @@ val nnrs_imp_to_sexp : QLang.nnrs_imp -> sexp
 val sexp_to_imp_qcert : sexp -> QLang.imp_qcert
 val imp_qcert_to_sexp : QLang.imp_qcert -> sexp
 
-val sexp_to_imp_json : sexp -> QLang.imp_json
-val imp_json_to_sexp : QLang.imp_json -> sexp
+val sexp_to_imp_ejson : sexp -> QLang.imp_ejson
+val imp_ejson_to_sexp : QLang.imp_ejson -> sexp
 
 
 val sexp_to_nnrcmr : sexp -> QLang.nnrcmr
