compiler/src/Common/Data/CommonData.v
@@ -18,7 +18,7 @@ Require Export Data.
 Require Export QResult.
 Require Export DataLift.
 Require Export DataNorm.
-Require Export DatatoEJSON.
+Require Export DatatoEJson.
 Require Export DataSort.
 Require Export DData.
 Require Export DDataNorm.
