compiler/src/Compiler/QLib/QUtil.v
@@ -54,7 +54,7 @@ Module QUtil(runtime:CompilerRuntime).
     Definition qfailure {fdata:foreign_data} (A:Set) : qerror -> qresult A := QResult.qfailure.
   End results.
 
-  Definition string_of_json_runtime_op := ImpJson.string_of_json_runtime_op.
+  Definition string_of_ejson_runtime_op := ImpEJson.string_of_ejson_runtime_op.
 
 End QUtil.
 
